refactoring, simplify proof a bit

theories/L/Complexity/Cook/BinaryPR_to_FSAT.v
@@ -6,9 +6,6 @@ From Undecidability.L.Datatypes Require Import Lists.
 
 Require Import Lia. 
 
-(*a generator type - given an index for the first variable to use, generate a formula *)
-Definition formulagen := nat -> formula. 
-
 Section fixInstance. 
   Variable (bpr : BinaryPR). 
   
@@ -24,6 +21,7 @@ Section fixInstance.
 
   Implicit Types (a : assgn) (v : var). 
 
+  (*convenience functions for creating formulas *)
   Notation Ffalse := (¬Ftrue). 
   Fixpoint listOr (l : list formula) := match l with
     | [] => Ffalse 
@@ -35,13 +33,12 @@ Section fixInstance.
     | a :: l => a ∧ listAnd l
     end.  
 
-  (*generate the list of values assigned to the variables in range [lower, lower + len) *)
+  (*generate the list of values assigned to the variables by a in range [lower, lower + len) *)
   Fixpoint explicitAssignment a lower len := 
     match len with
       | 0 => [] 
       | S len => explicitAssignment a lower len ++ [list_in_decb Nat.eqb a (lower + len)]
     end. 
-
 
   Lemma explicitAssignment_length a lower len : |explicitAssignment a lower len| = len. 
   Proof. 
@@ -61,19 +58,6 @@ Section fixInstance.
       + rewrite nth_error_app1; [ | rewrite explicitAssignment_length; easy ]. now apply IHlen. 
   Qed. 
 
-  Lemma explicitAssignment_lenO a s l : explicitAssignment a s l = [] <-> l = 0. 
-  Proof. 
-    specialize (explicitAssignment_length a s l). 
-    split; intros. 
-    - rewrite H0 in H. easy. 
-    - subst. destruct explicitAssignment; cbn in *; congruence. 
-  Qed. 
-
-  Corollary explicitAssignment_lenO' a l : explicitAssignment a l 0 = []. 
-  Proof. 
-    apply explicitAssignment_lenO. easy.
-  Qed. 
-
   Lemma explicitAssignment_app a l1 len1 len2: explicitAssignment a l1 (len1 + len2) = explicitAssignment a l1 len1 ++ explicitAssignment a (l1 + len1) len2. 
   Proof. 
     induction len2; cbn. 
@@ -81,655 +65,8 @@ Section fixInstance.
     - rewrite Nat.add_succ_r. cbn. rewrite IHlen2, app_assoc. easy. 
   Qed. 
 
-  Lemma explicitAssignment_length' a n: |explicitAssignment a 0 n| = n.
-  Proof. rewrite explicitAssignment_length. lia. Qed. 
-
-
-  Inductive varsInRange (min max : nat) : formula -> Prop := 
-    | varsInRangeTrue : varsInRange min max Ftrue
-    | varsInRangeVar v : v >= min -> v < max -> varsInRange min max v
-    | varsInRangeNeg f : varsInRange min max f -> varsInRange min max (¬f)
-    | varsInRangeAnd f1 f2 : varsInRange min max f1 -> varsInRange min max f2 -> varsInRange min max (f1 ∧ f2)
-    | varsInRangeOr f1 f2 : varsInRange min max f1 -> varsInRange min max f2 -> varsInRange min max (f1 ∨ f2). 
-
-  Hint Constructors varsInRange. 
-
-  Lemma varsInRange_monotonous (min1 max1 min2 max2 : nat) f : min2 <= min1 -> max2 >= max1 -> varsInRange min1 max1 f -> varsInRange min2 max2 f. 
-  Proof. intros. induction H1; eauto. constructor 2; lia. Qed. 
-
-  (*we define what it means for a formula to encode a predicate *)
-  Definition predicate := list bool -> Prop. 
-  Implicit Type (p : predicate).
-  Definition encodesPredicateAt (start : nat) (l : nat) f p:= 
-    varsInRange start (l + start) f /\ forall a, satisfies a f <-> p (explicitAssignment a start l). 
-
-  Definition projVars start len (l : list bool) := firstn len (skipn start l). 
-
-  Lemma projVars_length l s m : |l| >= (s + m) -> |projVars s m l| = m. 
-  Proof. 
-    intros. unfold projVars. rewrite firstn_length. rewrite skipn_length. lia. 
-  Qed. 
-
-  Lemma projVars_app1 l1 l2 m : |l1| = m -> projVars 0 m (l1 ++ l2) = l1.
-  Proof. 
-    intros. unfold projVars. cbn. rewrite firstn_app. subst. 
-    now rewrite Nat.sub_diag, firstn_O, app_nil_r, firstn_all.
-  Qed. 
-
-  Lemma projVars_app2 l1 l2 u m : |l1| = u -> projVars u m (l1 ++ l2) = projVars 0 m l2. 
-  Proof. 
-    intros. unfold projVars. rewrite skipn_app; [ | easy]. now cbn. 
-  Qed. 
-
-  Lemma projVars_app3 l1 l2 u1 u2 m : |l1| = u1 -> projVars (u1 + u2) m (l1 ++ l2) = projVars u2 m l2. 
-  Proof. 
-    intros. unfold projVars. erewrite skipn_add; [ easy| lia]. 
-  Qed. 
-
-  Lemma projVars_all l m : m = |l| -> projVars 0 m l = l. 
-  Proof.
-    intros. unfold projVars. cbn. rewrite H. apply firstn_all. 
-  Qed. 
-
-  (*encodings of two predicates can be combined*)
-  Definition combinedLength start1 start2 l1 l2 := max (start1 +l1) (start2 + l2) - min start1 start2. 
-  Definition combinedStart start1 start2 := min start1 start2. 
-
-  Lemma list_eq_nth_error (X : Type) (l1 l2 : list X) : 
-    l1 = l2 <-> (|l1| = |l2| /\ forall k, k < |l1| -> nth_error l1 k = nth_error l2 k). 
-  Proof. 
-    split; [intros -> | intros (H1 & H2)]. 
-    - split; [easy | intros; easy ]. 
-    - revert l2 H1 H2; induction l1; intros; destruct l2. 
-      + easy. 
-      + cbn in H1; congruence. 
-      + cbn in H1; congruence. 
-      + cbn in H1. apply Nat.succ_inj in H1. enough (a = x /\ l1 = l2) by easy; split. 
-        * specialize (H2 0 (Nat.lt_0_succ (|l1|))). now cbn in H2. 
-        * apply IHl1; [ apply H1 | ]. 
-          intros. apply Nat.succ_lt_mono in H. specialize (H2 (S k) H). now cbn in H2. 
-  Qed. 
-
-  Lemma nth_error_firstn (X : Type) k m (l : list X): k < m -> nth_error (firstn m l) k = nth_error l k. 
-  Proof. 
-    revert k l. induction m; intros. 
-    - lia.
-    - destruct k; cbn; destruct l; easy. 
-  Qed. 
-
-  Lemma nth_error_skipn (X : Type) k m (l : list X) : nth_error (skipn m l) k = nth_error l (m + k). 
-  Proof. 
-    revert k l. induction m; intros. 
-    - easy. 
-    - destruct l; cbn; [ now destruct k | apply IHm]. 
-  Qed. 
-
-  Lemma projVars_combined1 s1 s2 l1 l2 a: explicitAssignment a s1 l1 = projVars (s1 - combinedStart s1 s2) l1 (explicitAssignment a (combinedStart s1 s2) (combinedLength s1 s2 l1 l2)).
-  Proof. 
-    unfold projVars. 
-    apply list_eq_nth_error. split. 
-    - rewrite explicitAssignment_length. unfold combinedStart, combinedLength. rewrite firstn_length. 
-      rewrite skipn_length. rewrite explicitAssignment_length. lia. 
-    - intros. rewrite explicitAssignment_length in H. unfold combinedStart, combinedLength. 
-      rewrite nth_error_firstn; [ | apply H].  
-      rewrite nth_error_skipn. rewrite !explicitAssignment_nth; [easy | lia | lia]. 
-  Qed. 
-
-  Lemma projVars_combined2 s1 s2 l1 l2 a: explicitAssignment a s2 l2 = projVars (s2 - combinedStart s1 s2) l2 (explicitAssignment a (combinedStart s1 s2) (combinedLength s1 s2 l1 l2)). 
-  Proof. 
-    unfold combinedStart, combinedLength. rewrite Nat.min_comm. rewrite Nat.max_comm. apply projVars_combined1. 
-  Qed. 
-
-  Lemma encodesPredicate_and start1 start2 l1 l2 f1 f2 p1 p2 : 
-    encodesPredicateAt start1 l1 f1 p1 -> encodesPredicateAt start2 l2 f2 p2 
-    -> encodesPredicateAt (combinedStart start1 start2) (combinedLength start1 start2 l1 l2) (f1 ∧ f2) (fun m => (p1 (projVars (start1 - combinedStart start1 start2) l1 m) /\ p2 (projVars (start2 - combinedStart start1 start2) l2 m)) /\ |m| = combinedLength start1 start2 l1 l2). 
-  Proof. 
-    intros (G1 & G2) (F1 & F2). split. 
-    - constructor. 
-      + eapply varsInRange_monotonous; [ | | apply G1]; unfold combinedStart, combinedLength; lia. 
-      + eapply varsInRange_monotonous; [ | | apply F1]; unfold combinedStart, combinedLength; lia. 
-    - intros a. split; intros H. 
-      + apply evalFormula_and_iff in H as (H1%G2 & H2%F2). 
-        rewrite <- projVars_combined1, <- projVars_combined2, explicitAssignment_length. easy. 
-      + rewrite <- projVars_combined1, <- projVars_combined2 in H. 
-        unfold satisfies. apply evalFormula_and_iff. 
-        split; [apply G2, H | apply F2, H]. 
-  Qed. 
-
-  Lemma encodesPredicate_or start1 start2 l1 l2 f1 f2 p1 p2 : 
-    encodesPredicateAt start1 l1 f1 p1 -> encodesPredicateAt start2 l2 f2 p2 
-    -> encodesPredicateAt (combinedStart start1 start2) (combinedLength start1 start2 l1 l2) (f1 ∨ f2) (fun m => (p1 (projVars (start1 - combinedStart start1 start2) l1 m) \/ p2 (projVars (start2 - combinedStart start1 start2) l2 m)) /\ |m| = combinedLength start1 start2 l1 l2).
-  Proof. 
-    intros (G1 & G2) (F1 & F2). split. 
-    - constructor. 
-      + eapply varsInRange_monotonous; [ | | apply G1]; unfold combinedStart, combinedLength; lia. 
-      + eapply varsInRange_monotonous; [ | | apply F1]; unfold combinedStart, combinedLength; lia. 
-    - intros a. split; intros H. 
-      + split; [ | rewrite explicitAssignment_length; easy]. 
-        apply evalFormula_or_iff in H as [H1%G2 | H2%F2]. 
-        * left. rewrite <- projVars_combined1. apply H1.
-        * right. rewrite <- projVars_combined2. apply H2. 
-      + rewrite <- projVars_combined1, <- projVars_combined2 in H. 
-        destruct H as ([H | H] & _); apply evalFormula_or_iff; [left; apply G2, H | right; apply F2, H].  
-  Qed. 
-
-  (*encoding of single literals *)
-  Definition encodeLiteral v (sign : bool) : formula := if sign then v else ¬ v. 
-
-  Lemma encodeLiteral_correct v sign : forall a, satisfies a (encodeLiteral v sign) <-> evalVar a v = sign. 
-  Proof. 
-    intros. unfold satisfies, encodeLiteral. destruct sign; cbn; [ tauto |simp_bool; tauto ]. 
-  Qed. 
-
-  Lemma encodeLiteral_varsInRange v sign : varsInRange v (S v) (encodeLiteral v sign). 
-  Proof. 
-    unfold encodeLiteral. destruct sign; eauto. 
-  Qed. 
-
-  Lemma encodeLiteral_encodesPredicate v sign : encodesPredicateAt v 1 (encodeLiteral v sign) (fun l => l = [sign]). 
-  Proof. 
-    split. 
-    - apply encodeLiteral_varsInRange. 
-    - intros. split; intros. 
-      + apply encodeLiteral_correct in H. specialize (explicitAssignment_length a v 1) as H1. 
-        assert (0 < 1) as H2 by lia. 
-        specialize (@explicitAssignment_nth a v 1 0 H2) as H3. 
-        destruct explicitAssignment as [ | s l]; cbn in H1; [ congruence | destruct l; [ | cbn in H1; congruence]]. 
-        cbn in H3. now inv H3. 
-      + apply encodeLiteral_correct. assert (0 < 1) as H2 by lia.
-        specialize (@explicitAssignment_nth a v 1 0 H2) as H1. 
-        rewrite H in H1; cbn in H1. now inv H1. 
-  Qed. 
-
-  Lemma encodesPredicateAt_extensional s l f p1 p2 : (forall m, p1 m <-> p2 m) -> encodesPredicateAt s l f p1 <-> encodesPredicateAt s l f p2. 
-  Proof. 
-    intros. unfold encodesPredicateAt. setoid_rewrite H. easy. 
-  Qed. 
-  
-  (*encoding of lists *)
-  Fixpoint encodeListAt (startA : nat) (l : list bool) :=
-    match l with 
-    | [] => Ftrue
-    | x :: l => (encodeLiteral startA x) ∧ (encodeListAt (1 + startA) l)
-    end. 
-
-  Lemma firstn_all_inv (X : Type) (m l : list X) : |l| = |m| -> firstn (|l|) m = l -> m = l.
-  Proof. 
-    revert l; induction m; intros.
-    - destruct l; cbn; easy. 
-    - destruct l; cbn in *; [easy | ]. inv H0. apply Nat.succ_inj in H. 
-      rewrite H3. f_equal. now apply IHm. 
-  Qed. 
-
-  Lemma encodeListAt_encodesPredicate start l : encodesPredicateAt start (|l|) (encodeListAt start l) (fun m => m = l).
-  Proof. 
-    revert start. induction l; intros. 
-    - cbn. split; [eauto | ]. unfold satisfies.  
-      intros; split. 
-      + intros _. destruct start; now cbn. 
-      + intros _. easy. 
-    - cbn. specialize (@encodesPredicate_and start (S start) 1 (|l|) (encodeLiteral start a) (encodeListAt (S start) l) _ _ (encodeLiteral_encodesPredicate start a) (IHl (S start))) as H1.
-      replace (combinedStart start (S start)) with (start) in H1 by (unfold combinedStart; lia). 
-      replace (combinedLength start (S start) 1 (|l|)) with (S (|l|)) in H1 by (unfold combinedLength; lia). 
-      rewrite Nat.sub_diag in H1. replace (S start - start) with 1 in H1 by lia. 
-      eapply encodesPredicateAt_extensional; [ | apply H1]. 
-      intros. unfold projVars. 
-      destruct m; cbn; [split; intros; easy | ]. 
-      split. 
-      + intros H. inv H. now rewrite firstn_all.
-      + intros ((H0 & H2) & H3). inv H0. f_equal. apply Nat.succ_inj in H3. 
-        now apply firstn_all_inv. 
-  Qed. 
-
-  Ltac encodesPredicateAt_comp_simp H := 
-    unfold combinedStart, combinedLength in H;
-    try (rewrite Nat.min_l in H by nia); try (rewrite Nat.min_r in H by nia);
-    try (rewrite Nat.max_l in H by nia); try (rewrite Nat.max_r in H by nia);
-    try rewrite !Nat.sub_diag in H; cbn -[projVars] in H.
-
-  (*encoding of windows *)
-  Definition encodeWindowAt (startA startB : nat) (win : PRWin bool) := encodeListAt startA (prem win) ∧ encodeListAt startB (conc win). 
-  Lemma encodeWindowAt_encodesPredicate start len win : win el windows -> encodesPredicateAt start (len + width) (encodeWindowAt start (start + len) win) (fun m => projVars 0 width m = prem win /\ projVars len width m = conc win /\ |m| = len + width). 
-  Proof. 
-    intros H0. 
-    specialize (encodesPredicate_and (encodeListAt_encodesPredicate start (prem win)) (encodeListAt_encodesPredicate (start + len) (conc win))) as H. 
-    destruct A as (_ & _ & _ & A0 & A1 & _). apply A1 in H0 as (H0 & H0').
-    encodesPredicateAt_comp_simp H. 
-    rewrite !H0 in H. rewrite !H0' in H.
-    replace (start + len + width - start) with (len + width) in H by lia. 
-    replace (start + len - start) with len in H by lia.
-    unfold encodeWindowAt. eapply encodesPredicateAt_extensional; [ | apply H].
-    tauto.
-  Qed.
-
-  Definition encodeWindowsAt (startA startB : nat) := listOr (map (encodeWindowAt startA startB) windows). 
-
-  Lemma skipn_firstn_shift (X : Type) (m : list X) len l : skipn l (firstn len m) = firstn (len - l) (skipn l m). 
-  Proof. 
-    revert l len. induction m; cbn; intros. 
-    - rewrite !firstn_nil, !skipn_nil, firstn_nil. easy. 
-    - destruct len. 
-      + cbn. now destruct l.
-      + cbn. destruct l; cbn; [ easy | ]. now rewrite IHm. 
-  Qed. 
-
-  Lemma skipn_skipn (X : Type) (m : list X) l1 l2 : skipn l1 (skipn l2 m) = skipn (l1 + l2) m. 
-  Proof. 
-    revert l1 l2. 
-    induction m; intros; destruct l2; cbn; try now rewrite !skipn_nil. 
-    - now rewrite Nat.add_0_r. 
-    - rewrite IHm. rewrite Nat.add_succ_r. easy. 
-  Qed. 
-
-  Lemma skipn_firstn_skipn (X : Type) (m : list X) l1 l2 len2 : 
-    skipn l1 (firstn len2 (skipn l2 m)) = firstn (len2 - l1) (skipn (l1 + l2) m). 
-  Proof. 
-    intros. 
-    rewrite skipn_firstn_shift. now rewrite skipn_skipn. 
-  Qed. 
-
-  Lemma projVars_comp l1 l2 len1 len2 m: projVars l1 len1 (projVars l2 len2 m) = projVars (l1 + l2) (min len1 (len2 - l1)) m. 
-  Proof. 
-    unfold projVars. intros. 
-    rewrite skipn_firstn_skipn. rewrite firstn_firstn. reflexivity. 
-  Qed. 
-
-  Lemma encodeWindowsAt_encodesPredicate len start : len >= width -> encodesPredicateAt start (len + width) (encodeWindowsAt start (start + len)) (fun m => exists win, win el windows /\ projVars 0 width m = prem win /\ projVars len width m = conc win /\ |m| = len + width). 
-  Proof. 
-    intros F0.
-    specialize (encodeWindowAt_encodesPredicate) as H1. 
-    unfold encodeWindowsAt. 
-    induction windows. 
-    - cbn. split. 
-      + eauto. 
-      + intros; split. 
-        * unfold satisfies. cbn. congruence. 
-        * intros (win & [] & _). 
-    - cbn. match type of IHl with ?a -> _ => assert a as H by (intros; apply H1; eauto); apply IHl in H; clear IHl end. 
-      specialize (H1 start len a (or_introl eq_refl)). 
-      specialize (encodesPredicate_or H1 H) as H2. clear H1 H. 
-      cbn in H2. 
-      destruct A as (_ & _ & (k & A1 & A2) & _).
-      encodesPredicateAt_comp_simp H2. 
-      replace (start + (len + width) - start) with (len + width) in H2 by lia.
-      eapply encodesPredicateAt_extensional; [ | apply H2]. 
-      intros; cbn. 
-      rewrite !projVars_comp. cbn. rewrite !Nat.min_l by lia. rewrite Nat.add_0_r. split; intros. 
-      + destruct H as (win & [<- | H] & F1 & F2 & F3); (rewrite projVars_length; [ split; [ | easy] | easy]); [now left | right; eauto].
-      + destruct H as ([(F1 & F2 & F3) | (win & H & F1 & F2 & F3)] & F4); eauto 7. 
-  Qed. 
-
-  (*we only need to place a window every offset fields, but subtracting offset isn't structurally recursive *)
-  (*therefore we use a stepindex (initalise to the same value as l) *)
-  Fixpoint encodeWindowsInLine' (stepindex l : nat) (startA startB : nat) := 
-    if l <? width then Ftrue 
-                  else match stepindex with 
-                    | 0 => Ftrue
-                    | S stepindex => encodeWindowsAt startA startB ∧ encodeWindowsInLine' stepindex (l - offset) (startA + offset) (startB + offset)
-                    end.
-
-  Lemma encodeWindowsInLine'_stepindex_monotone' index startA startB : forall n, n <= index -> encodeWindowsInLine' index n startA startB = encodeWindowsInLine' (S index) n startA startB. 
-  Proof. 
-    destruct A as (A1 & A2 & _).
-    revert startA startB.
-    induction index; intros. 
-    - unfold encodeWindowsInLine'. assert (n = 0) as -> by lia. cbn; destruct width; [ lia | easy ].
-    - unfold encodeWindowsInLine'. destruct (Nat.ltb n width); [ easy | ]. fold encodeWindowsInLine'. 
-      erewrite IHindex by lia. easy. 
-  Qed. 
-
-  Lemma encodeWindowsInLine'_stepindex_monotone index index' startA startB : index' >= index -> encodeWindowsInLine' index index startA startB = encodeWindowsInLine' index' index startA startB. 
-  Proof. 
-    intros. revert index H.
-    induction index'; intros. 
-    - assert (index = 0) as -> by lia. easy.
-    - destruct (nat_eq_dec (S index') index). 
-      + now rewrite e.
-      + assert (index' >= index) as H1 by lia. rewrite <- encodeWindowsInLine'_stepindex_monotone' by lia. now apply IHindex'.
-  Qed.
-
-  Lemma firstn_add (X : Type) (m : list X) l1 l2 : firstn (l1 + l2) m = firstn l1 m ++ firstn l2 (skipn l1 m). 
-  Proof. 
-    revert l1 l2. induction m; intros. 
-    - now rewrite !skipn_nil, !firstn_nil.
-    - destruct l1; cbn; [ easy | ]. now rewrite IHm. 
-  Qed. 
-
-  Lemma projVars_add s l1 l2 m : projVars s (l1 + l2) m = projVars s l1 m ++ projVars (s + l1) l2 m. 
-  Proof. 
-    unfold projVars. rewrite firstn_add, skipn_skipn. now rewrite Nat.add_comm. 
-  Qed.
-
-  Lemma encodeWindowsInLine'_encodesPredicate start l : l <= llength -> (exists k, l = k * offset) -> encodesPredicateAt start (l + llength) (encodeWindowsInLine' l l start (start + llength)) (fun m => valid offset width windows (projVars 0 l m) (projVars llength l m) /\ |m| = l + llength). 
-  Proof. 
-    intros A0.
-    (*need strong induction *)
-    destruct A as (A1 & A4 & A2 & A5 & A7 & A3). 
-    revert start A0.  
-    apply complete_induction with (x := l). clear l. intros l IH. intros. 
-
-    destruct l.
-    - cbn. destruct width; [ lia | ]. split; [eauto | ]. 
-      intros a. split; [ intros; split; [constructor | ] | intros _; unfold satisfies; eauto]. now rewrite explicitAssignment_length. 
-    - destruct (le_lt_dec width (S l)). 
-      + assert (~ (S l) < width) as H3%Nat.ltb_nlt by lia. cbn -[projVars]; setoid_rewrite H3. 
-        destruct offset as [ | offset]; [ lia | ].
-        (* we use the IH for l - offset *)
- 
-        assert (S l - S offset < S l) as H1 by lia. apply IH with (start := start + S offset) in H1. 2: nia. 
-        2: { destruct H as (k & H). destruct k; [ lia | ]. exists k. lia. }
-        clear H IH. 
-        assert (llength >= width) as H0 by lia.
-        apply (encodeWindowsAt_encodesPredicate start) in H0. 
-        specialize (encodesPredicate_and H0 H1) as H2. clear H1 H0.
-        encodesPredicateAt_comp_simp H2. 
-        replace (start + S offset + llength) with (start + llength + S offset) in H2 by lia. 
-        replace (start + S offset + (l - offset + llength) - start) with (S (l + llength)) in H2. 
-        2: { destruct A2 as (? & A2 & A6). nia. }
-        
-        rewrite encodeWindowsInLine'_stepindex_monotone with (index' := l) in H2; [ | lia].
-        eapply encodesPredicateAt_extensional; [ | apply H2].
-        clear H2 H3. 
-        intros. 
-        destruct A2 as (k & A2 & A2').
-        assert (S l = S offset + (S l - S offset)) as H by nia.  
-        split; intros. 
-        * destruct H0 as (H1 & H2). rewrite projVars_length; [ | easy]. 
-          rewrite H in H1. clear H. 
-          rewrite !projVars_add in H1. inv H1.
-          2 : { exfalso. apply list_eq_length in H. rewrite !app_length in H. rewrite !projVars_length in H; [ | easy | easy]. nia. }
-          1: { exfalso. apply list_eq_length in H0. rewrite !app_length in H0. rewrite projVars_length in H0; [ | cbn; nia]. cbn in H0. lia. } 
-
-          apply app_eq_length in H as (-> & ->); [ | rewrite projVars_length; [easy | nia] ].
-          apply app_eq_length in H0 as (-> & ->); [ | rewrite projVars_length; [easy | nia]]. 
-          specialize (@projVars_length m 0 (S l)) as H8.
-          rewrite projVars_length; [ | nia]. split; [ split; [ | split; [ | easy]] | easy]; clear H8.
-          -- exists win. rewrite !projVars_comp; cbn. rewrite !Nat.min_l by lia. 
-             rewrite !Nat.add_0_r.
-             clear H3 H4 H5. rewrite <- !projVars_add in H7. 
-             replace (S offset + (l - offset)) with (width + (S l - width)) in H7 by nia. 
-             rewrite !projVars_add in H7.
-             split; [ easy | split; [ | split; [ | easy]]]; apply A7 in H6 as (H6 & H6'). 
-             ++ destruct H7 as ((b & H7) & _). eapply app_eq_length in H7; [ easy| rewrite projVars_length; easy ]. 
-             ++ destruct H7 as (_ & (b & H7)). eapply app_eq_length in H7; [ easy | rewrite projVars_length; easy].
-          -- clear H7 H6. 
-             rewrite projVars_comp. cbn. replace (start + S offset - start) with (S offset) by lia. rewrite Nat.min_l by lia. 
-             rewrite projVars_comp. cbn. rewrite Nat.min_l by lia. 
-             apply H3. 
-        * (*other direction of the equivalence *)
-          destruct H0 as ((H1  & (H2 & H3)) & H4). split; [ | apply H4]. 
-          rewrite H. rewrite !projVars_add. 
-          destruct H1 as (win & H1 & F1 & F2 & _). 
-          econstructor 3. 
-          -- clear H1. rewrite !projVars_comp in H2. rewrite !Nat.min_l in H2 by lia.
-             replace (start + S offset - start) with (S offset) in H2 by lia. 
-             apply H2. 
-          -- rewrite projVars_length; lia. 
-          -- rewrite projVars_length; lia. 
-          -- clear H2. apply H1. 
-          -- clear H2. rewrite <- !projVars_add. 
-             replace (S offset + (S l - S offset)) with (width + (S l - width)) by lia. 
-             rewrite !projVars_add. 
-             rewrite projVars_comp in F1, F2. rewrite !Nat.min_l in F1, F2 by lia. 
-             rewrite Nat.add_0_r in F2; cbn in F1, F2.
-             rewrite F1, F2. split; unfold prefix; eauto. 
-    + (*the case where the remaining string is too short for a rewrite window to hold - validity holds vacuously *)
-      clear IH. assert ( (S l) < width) as H3%Nat.ltb_lt by lia. cbn -[projVars]; setoid_rewrite H3.
-      split; [eauto | ]. unfold satisfies; cbn [evalFormula]. setoid_rewrite explicitAssignment_length. 
-      intros a; split; [intros _ | ]. 
-      * split; [ | easy]. destruct H as (k & H). eapply valid_vacuous. 
-        -- rewrite !projVars_length; [easy | rewrite explicitAssignment_length; lia | rewrite explicitAssignment_length; lia]. 
-        -- rewrite projVars_length; [ easy | rewrite explicitAssignment_length; lia]. 
-        -- rewrite projVars_length; [ | rewrite explicitAssignment_length; lia]. 
-           (*here we need the assumption that l is a multiple of offset *)
-           apply H. 
-      * intros _; easy. 
-  Qed.
-
-  Definition encodeWindowsInLine start := encodeWindowsInLine' llength llength start (start + llength). 
-  Lemma encodeWindowsInLine_encodesPredicate start : encodesPredicateAt start (llength + llength) (encodeWindowsInLine start) (fun m => valid offset width windows (projVars 0 llength m) (projVars llength llength m) /\ |m| = llength + llength). 
-  Proof. 
-    unfold encodeWindowsInLine.
-    apply (@encodeWindowsInLine'_encodesPredicate start llength); [easy | apply A].
-  Qed. 
-
-  Fixpoint encodeWindowsInAllLines' (start : nat) (t : nat)  := 
-    match t with 
-    | 0 => Ftrue
-    | S t => encodeWindowsInLine start ∧ encodeWindowsInAllLines' (start + llength) t
-    end. 
-
-  Definition encodeWindowsInAllLines := encodeWindowsInAllLines' 0 steps. 
-
-  Lemma encodeWindowsInAllLines'_encodesPredicate start : encodesPredicateAt start ((S steps) * llength) (encodeWindowsInAllLines' start steps) 
-    (fun m => (forall i, 0 <= i < steps -> valid offset width windows (projVars (i * llength) llength m) (projVars (S i * llength) llength m)) /\ |m| = (S steps) * llength). 
-  Proof. 
-    revert start. induction steps; cbn; intros. 
-    - split; [ easy | ]. rewrite !Nat.add_0_r. 
-      intros a; unfold satisfies; cbn; split; [ intros _; split; [intros; lia | rewrite explicitAssignment_length; lia]| easy]. 
-    - specialize (encodeWindowsInLine_encodesPredicate start) as H1. 
-      specialize (IHn (start + llength)). 
-      specialize (encodesPredicate_and H1 IHn) as H. clear IHn H1. 
-      encodesPredicateAt_comp_simp H. 
-      replace (start + llength + S n * llength - start) with (llength + (llength + n * llength)) in H by lia. 
-      replace (start + llength - start) with llength in H by lia. 
-      eapply encodesPredicateAt_extensional; [ | apply H].
-      clear H. intros m. cbn -[projVars]. 
-      rewrite !projVars_comp. setoid_rewrite projVars_comp. cbn. rewrite !Nat.min_l by lia. 
-      rewrite Nat.add_0_r. split. 
-      + intros (H1 & H2). split; [ split |  easy]. 
-        * specialize (H1 0). cbn in H1. rewrite Nat.add_0_r in H1. split; [apply H1; lia | now rewrite projVars_length].
-        * split; [ | now rewrite projVars_length]. intros i H. 
-          specialize (H1 (S i)). cbn in H1. rewrite Nat.add_comm. rewrite <- Nat.add_assoc. 
-          rewrite !Nat.min_l by nia.
-          setoid_rewrite Nat.add_comm at 3.
-          apply H1. lia.
-      + intros ((H1 & (H2 & _)) & H3). split; [ clear H3| apply H3]. intros i H. 
-        destruct i. 
-        * cbn. rewrite Nat.add_0_r. apply H1.
-        * specialize (H2 i). 
-          rewrite !Nat.min_l in H2 by nia.
-          cbn. rewrite Nat.add_comm. rewrite Nat.add_assoc. now apply H2. 
-  Qed.
-
-  Corollary encodeWindowsInAllLines_encodesPredicate : encodesPredicateAt 0 ((S steps) * llength) encodeWindowsInAllLines 
-    (fun m => (forall i, 0 <= i < steps -> valid offset width windows (projVars (i * llength) llength m) (projVars (S i * llength) llength m)) /\ |m| = (S steps) * llength). 
-  Proof. 
-    unfold encodeWindowsInAllLines. apply encodeWindowsInAllLines'_encodesPredicate. 
-  Qed. 
-
-  (*should only be called for s satisfying |s| > 0; for s = nil, the breaking condition does not work as intended*)
-  (*in principle, this is not a problem as the resulting formula is still equivalent to the desired formula, but this breaks monotonicity*)
-  Fixpoint encodeSubstringInLine' (s : list bool) (stepindex l : nat) (start : nat) := 
-    if l <? |s| then Ffalse
-                  else match stepindex with 
-                    | 0 => (match s with [] => Ftrue | _ => Ffalse end)
-                    | S stepindex => encodeListAt start s ∨ encodeSubstringInLine' s stepindex (l - offset) (start + offset) 
-                    end.
-
-  Lemma encodeSubstringInLine'_stepindex_monotone' s index start : forall n, |s| > 0 -> n <= index -> encodeSubstringInLine' s index n start = encodeSubstringInLine' s (S index) n start. 
-  Proof. 
-    destruct A as (A1 & A2 & _).
-    revert start.
-    induction index; intros. 
-    - unfold encodeSubstringInLine'. assert (n = 0) as -> by lia. cbn; destruct s; [ cbn in *; lia | easy ]. 
-    - unfold encodeSubstringInLine'. destruct (Nat.ltb n (|s|)); [ easy | ]. fold encodeSubstringInLine'. 
-      erewrite IHindex by lia. easy. 
-  Qed. 
-
-  Lemma encodeSubstringInLine'_stepindex_monotone s index1 index2 start : 
-    |s| > 0 -> index2 >= index1 -> encodeSubstringInLine' s index1 index1 start = encodeSubstringInLine' s index2 index1 start.
-  Proof. 
-    intros. revert index1 H0. 
-    induction index2; intros.
-    - assert (index1 = 0) as -> by lia. easy.
-    - destruct (nat_eq_dec (S index2) index1). 
-      + now rewrite e.
-      + assert (index2 >= index1) as H1 by lia. rewrite <- encodeSubstringInLine'_stepindex_monotone' by lia. now apply IHindex2.
-  Qed. 
-
-  Lemma projVars_length_le start l m: |projVars start l m| <= |m|. 
-  Proof. 
-    unfold projVars. 
-    rewrite firstn_length. rewrite skipn_length. lia. 
-  Qed. 
-
-  Lemma projVars_length_le2 start l m : |projVars start l m| <= l.
-  Proof. 
-    unfold projVars. rewrite firstn_length, skipn_length. lia. 
-  Qed. 
-
-  Lemma projVars_in_ge start l m : start <= |m| -> projVars start (|l|) m = l -> |m| >= start + |l|. 
-  Proof. 
-    intros H0 H. unfold projVars in H. rewrite <- H, firstn_length, skipn_length. lia.
-  Qed. 
-
-  Lemma encodeSubstringInLine'_encodesPredicate s start l : |s| > 0 -> l <= llength -> (exists k, l = k * offset) -> encodesPredicateAt start l (encodeSubstringInLine' s l l start) (fun m => (exists k, k * offset <= l /\ projVars (k * offset) (|s|) m = s) /\ |m| = l). 
-  Proof. 
-    intros F.
-    (*need strong induction *)
-    destruct A as (A1 & A4 & A2 & A5 & A7 & A3). 
-    revert start.  
-    apply complete_induction with (x := l). clear l. intros l IH. intros. 
-
-    destruct l.
-    - cbn -[projVars]. destruct s; cbn -[projVars]. 
-      + (*trivially true *) split; [ easy | intros; unfold satisfies; cbn; split; intros _; eauto].
-        split; [exists 0; split; [lia | easy] | easy ].
-      + (*trivially false *)
-        split; [ easy | ]. intros a; split.
-        * unfold satisfies; cbn; congruence. 
-        * intros ((k & H1 & H2) & _). destruct k; [clear H1 | nia].
-          cbn in H2. congruence. 
-    - destruct (le_lt_dec (|s|) (S l)). 
-      + assert (~ (S l) < (|s|)) as H3%Nat.ltb_nlt by lia. cbn -[projVars]; setoid_rewrite H3. 
-        destruct offset as [ | offset]; [ lia | ].
-        (* we use the IH for l - offset *)
- 
-        assert (S l - S offset < S l) as H1 by lia. apply IH with (start := start + S offset) in H1. 2: nia. 
-        2: { destruct H0 as (k & H0). destruct k; [ lia | ]. exists k. lia. }
-        clear H IH. 
-        specialize (encodeListAt_encodesPredicate start s) as H2.
-        specialize (encodesPredicate_or H2 H1) as H. clear H1 H2 H3.
-        encodesPredicateAt_comp_simp H.
-        destruct H0 as (k & H0).
-        assert (k > 0) by nia. (*a hint for nia - without it, the following replace will not work *)
-        replace (start + S offset + (S l - S offset) - start) with (S l) in H by nia.
-        replace (start + S offset - start) with (S offset) in H by lia.
-
-        rewrite encodeSubstringInLine'_stepindex_monotone with (index2 := l) in H; [ | apply F| lia].
-        eapply encodesPredicateAt_extensional; [ | apply H]. clear H.
-        intros. cbn. split.
-        * intros ((k0 & H2 & H3) & H4). split; [ | easy]. 
-          destruct k0; [ now left | right]. 
-          split; [ | rewrite projVars_length; [ easy | nia] ]. 
-          exists (k0). split; [ easy | ]. 
-          rewrite projVars_comp. 
-          cbn [Nat.mul] in H3.  
-          enough (|s| <= l - offset - k0 * S offset).
-          { rewrite Nat.min_l by lia. rewrite Nat.add_comm. apply H3. }
-          apply projVars_in_ge in H3; nia.
-        * intros (H & H2). split; [ | apply H2]. 
-          destruct H as [H | (H & _)]; [ exists 0; cbn; easy | ]. 
-          destruct H as (k0 & H & H'). 
-          exists (S k0). split; [ nia | ].
-          rewrite projVars_comp in H'. 
-
-          enough (|s| <= l - offset - k0 * S offset).
-          { rewrite Nat.min_l in H' by lia. cbn [Nat.mul]. rewrite <- Nat.add_comm. apply H'. }
-          apply list_eq_length in H'. 
-          match type of H' with (|projVars ?a ?b ?c| = _) => specialize (projVars_length_le2 a b c) as H3 end.
-          lia. 
-    + (*the case where the remaining string is too short in order to place the substring constraint *)
-      clear IH. assert ( (S l) < (|s|)) as H3%Nat.ltb_lt by lia. cbn -[projVars]; setoid_rewrite H3.
-      split; [eauto | ]. unfold satisfies; cbn [negb evalFormula]. setoid_rewrite explicitAssignment_length. 
-      intros a; split; [congruence | ]. 
-      intros ((k & H1 & H2) & _). 
-      apply list_eq_length in H2. specialize (projVars_length_le (k * offset) (|s|) (explicitAssignment a start (S l))) as H4.
-      rewrite explicitAssignment_length in H4. lia. 
-  Qed.
-
-  (*TODO: consistent argument order over all functions *)
-  Definition encodeSubstringInLine s start l := match s with [] => Ftrue | _ => encodeSubstringInLine' s l l start end.
-  Lemma encodeSubstringInLine_encodesPredicate s start l : l <= llength -> (exists k, l = k * offset) -> encodesPredicateAt start l (encodeSubstringInLine s start l) (fun m => (exists k, k * offset <= l /\ projVars (k * offset) (|s|) m = s) /\ |m| = l). 
-  Proof. 
-    intros. unfold encodeSubstringInLine. destruct s eqn:H1. 
-    - split; [easy | ]. unfold satisfies. cbn. intros; split.
-      + intros _. split; [exists 0; cbn; firstorder |now rewrite explicitAssignment_length  ]. 
-      + intros _. reflexivity. 
-    - apply encodeSubstringInLine'_encodesPredicate; cbn; easy.
-  Qed. 
-
-  Definition encodeFinalConstraint (start : nat) := listOr (map (fun s => encodeSubstringInLine s start llength) final). 
-
-  Lemma encodesPredicate_listOr (X : Type) (l : list X) (encode : X -> nat -> nat -> formula) (p : X -> list bool -> Prop) start len : 
-    (forall x, x el l -> encodesPredicateAt start len (encode x start len) (p x)) 
-   -> encodesPredicateAt start len (listOr (map (fun x => encode x start len) l)) (fun m => (exists x, x el l /\ p x m) /\ |m| = len). 
-  Proof. 
-    intros H. induction l. 
-    - cbn. split; [easy | ]. unfold satisfies; cbn. intros a; split; [ congruence | intros ((_ & [] & _) & _)]. 
-    - specialize (IHl (fun x Hel => H x (or_intror Hel))). cbn. 
-      specialize (H a (or_introl eq_refl)). 
-      specialize (encodesPredicate_or H IHl) as H1. clear IHl H. 
-      encodesPredicateAt_comp_simp H1. 
-      replace (start + len - start) with len in H1 by lia. 
-
-      eapply encodesPredicateAt_extensional; [ clear H1| apply H1].
-      intros; split.
-      + intros ((x & [-> | H] & H1) & H2); (split; [ | easy]). 
-        * left; now rewrite projVars_all.
-        * right. rewrite projVars_length, projVars_all; easy. 
-      + intros ([H | ((x & H & H') & H1)] & H2); (split; [ | easy]).
-        * exists a. now rewrite projVars_all in H.
-        * exists x. rewrite projVars_length in H1; [ | easy]. rewrite projVars_all in H'; easy.
-  Qed. 
-
-  Lemma encodeFinalConstraint_encodesPredicate start : encodesPredicateAt start llength (encodeFinalConstraint start) (fun m => satFinal offset llength final m /\ |m| = llength).
-  Proof. 
-    unfold encodeFinalConstraint. 
-    eapply encodesPredicateAt_extensional; [ | apply encodesPredicate_listOr]. 
-    2: { intros. apply encodeSubstringInLine_encodesPredicate; [easy | apply A]. }
-    intros. split. 
-    - intros ((subs & k & H1 & H2 & H3) & H4). split; [ | easy].
-      exists subs. split; [ apply H1 | split; [ | apply H4]]. 
-      exists k. split; [ easy | ]. 
-      destruct H3 as (b & H3). unfold projVars. rewrite H3. 
-      rewrite firstn_app, firstn_all, Nat.sub_diag; cbn. now rewrite app_nil_r. 
-    - intros ((subs & H1 & (k & H2 & H3) & H4) & _). split; [ | apply H4].
-      exists subs, k. split; [apply H1 | split; [ apply H2 | ]].
-      unfold prefix. unfold projVars in H3. 
-      setoid_rewrite <- firstn_skipn with (l := skipn (k * offset) m) (n:= |subs|).
-      setoid_rewrite H3. eauto.
-  Qed. 
-
-  Definition encodeTableau := encodeListAt 0 init ∧ encodeWindowsInAllLines ∧ encodeFinalConstraint (steps * llength).
-  Lemma encodeTableau_encodesPredicate : 
-    encodesPredicateAt 0 (S steps * llength) encodeTableau 
-    (fun m => projVars 0 llength m = init 
-      /\ (forall i, 0 <= i < steps -> valid offset width windows (projVars (i * llength) llength m) (projVars (S i * llength) llength m)) 
-      /\ satFinal offset llength final (projVars (steps * llength) llength m)
-      /\ |m| = (S steps * llength)). 
-  Proof. 
-    specialize (encodesPredicate_and (encodeListAt_encodesPredicate 0 init) encodeWindowsInAllLines_encodesPredicate) as H. 
-    encodesPredicateAt_comp_simp H.  
-    specialize (encodesPredicate_and H (encodeFinalConstraint_encodesPredicate (steps * llength))) as H1.
-    clear H. 
-    encodesPredicateAt_comp_simp H1. 
-    unfold encodeTableau. 
-    replace (llength + steps * llength - 0 - 0) with (S steps * llength) in H1 by lia.
-
-    eapply encodesPredicateAt_extensional; [ clear H1| apply H1].
-    intros m; cbn. rewrite !projVars_comp. setoid_rewrite projVars_comp.
-    rewrite !Nat.min_l by nia. cbn. 
-    setoid_rewrite Nat.add_0_r. setoid_rewrite Nat.sub_0_r. 
-    split. 
-    - intros (H1 & H2 & H3 & H4). 
-      repeat split; try (rewrite projVars_length; nia); try nia; [easy | | easy].
-      intros. rewrite !Nat.min_l by nia. now apply H2.
-    - rewrite !and_assoc. intros (H1 & H2 & (_ & _ & H3 & _ & H4)); split; [easy |split;[ | easy]]. 
-      intros. specialize (H2 i H). rewrite !Nat.min_l in H2 by nia. apply H2.
-  Qed. 
-
+  (*from an explicit assignment, we can go back to an assignment *)
+  (*s is the variable index at which the explicit assignment is starting *)
   Lemma expAssgn_to_assgn s b : 
     {a & forall x, x el a <-> x >= s /\ nth_error b (x - s) = Some true}.
   Proof. 
@@ -766,8 +103,583 @@ Section fixInstance.
       + destruct b0; [ | easy]. exfalso; apply H2. apply H. 
         replace (s + k - s) with k by lia. easy.
       + apply nth_error_none in H3. lia.
+  Qed.
+
+  (*we define what it means for a formula to encode a predicate *)
+  Definition predicate := list bool -> Prop. 
+  Implicit Type (p : predicate).
+  Definition encodesPredicateAt (start : nat) (l : nat) f p:= forall a, satisfies a f <-> p (explicitAssignment a start l). 
+
+  (*given an explicitAssignment, we can project out a range of variables, given by [start, start+len) *)
+  Definition projVars start len (l : list bool) := firstn len (skipn start l). 
+
+  Lemma projVars_length l s m : |l| >= (s + m) -> |projVars s m l| = m. 
+  Proof. 
+    intros. unfold projVars. rewrite firstn_length. rewrite skipn_length. lia. 
   Qed. 
 
+  Lemma projVars_app1 l1 l2 m : |l1| = m -> projVars 0 m (l1 ++ l2) = l1.
+  Proof. 
+    intros. unfold projVars. cbn. rewrite firstn_app. subst. 
+    now rewrite Nat.sub_diag, firstn_O, app_nil_r, firstn_all.
+  Qed. 
+
+  Lemma projVars_app2 l1 l2 u m : |l1| = u -> projVars u m (l1 ++ l2) = projVars 0 m l2. 
+  Proof. 
+    intros. unfold projVars. rewrite skipn_app; [ | easy]. now cbn. 
+  Qed. 
+
+  Lemma projVars_app3 l1 l2 u1 u2 m : |l1| = u1 -> projVars (u1 + u2) m (l1 ++ l2) = projVars u2 m l2. 
+  Proof. 
+    intros. unfold projVars. erewrite skipn_add; [ easy| lia]. 
+  Qed. 
+
+  Lemma projVars_all l m : m = |l| -> projVars 0 m l = l. 
+  Proof.
+    intros. unfold projVars. cbn. rewrite H. apply firstn_all. 
+  Qed. 
+
+  Lemma projVars_comp l1 l2 len1 len2 m: projVars l1 len1 (projVars l2 len2 m) = projVars (l1 + l2) (min len1 (len2 - l1)) m. 
+  Proof. 
+    unfold projVars. intros. 
+    rewrite skipn_firstn_skipn. rewrite firstn_firstn. reflexivity. 
+  Qed. 
+
+  Lemma projVars_add s l1 l2 m : projVars s (l1 + l2) m = projVars s l1 m ++ projVars (s + l1) l2 m. 
+  Proof. 
+    unfold projVars. rewrite firstn_add, skipn_skipn. now rewrite Nat.add_comm. 
+  Qed.
+
+  Lemma projVars_length_le start l m: |projVars start l m| <= |m|. 
+  Proof. 
+    unfold projVars. 
+    rewrite firstn_length. rewrite skipn_length. lia. 
+  Qed. 
+
+  Lemma projVars_length_le2 start l m : |projVars start l m| <= l.
+  Proof. 
+    unfold projVars. rewrite firstn_length, skipn_length. lia. 
+  Qed. 
+
+  Lemma projVars_in_ge start l m : start <= |m| -> projVars start (|l|) m = l -> |m| >= start + |l|. 
+  Proof. 
+    intros H0 H. unfold projVars in H. rewrite <- H, firstn_length, skipn_length. lia.
+  Qed. 
+
+  (*encodings of two predicates can be combined*)
+  Definition combinedLength start1 start2 l1 l2 := max (start1 +l1) (start2 + l2) - min start1 start2. 
+  Definition combinedStart start1 start2 := min start1 start2. 
+
+  (*from the combined assignment for the combination of two formulas, we can restore an assigment for the first formula *)
+  Lemma projVars_combined1 s1 s2 l1 l2 a: explicitAssignment a s1 l1 = projVars (s1 - combinedStart s1 s2) l1 (explicitAssignment a (combinedStart s1 s2) (combinedLength s1 s2 l1 l2)).
+  Proof. 
+    unfold projVars. 
+    apply list_eq_nth_error. split. 
+    - rewrite explicitAssignment_length. unfold combinedStart, combinedLength. rewrite firstn_length. 
+      rewrite skipn_length. rewrite explicitAssignment_length. lia. 
+    - intros. rewrite explicitAssignment_length in H. unfold combinedStart, combinedLength. 
+      rewrite nth_error_firstn; [ | apply H].  
+      rewrite nth_error_skipn. rewrite !explicitAssignment_nth; [easy | lia | lia]. 
+  Qed. 
+
+  (*...and for the second *)
+  Lemma projVars_combined2 s1 s2 l1 l2 a: explicitAssignment a s2 l2 = projVars (s2 - combinedStart s1 s2) l2 (explicitAssignment a (combinedStart s1 s2) (combinedLength s1 s2 l1 l2)). 
+  Proof. 
+    unfold combinedStart, combinedLength. rewrite Nat.min_comm. rewrite Nat.max_comm. apply projVars_combined1. 
+  Qed. 
+
+  (*two formulae can be combined via ∧ *)
+  Lemma encodesPredicate_and start1 start2 l1 l2 f1 f2 p1 p2 : 
+    encodesPredicateAt start1 l1 f1 p1 -> encodesPredicateAt start2 l2 f2 p2 
+    -> encodesPredicateAt (combinedStart start1 start2) (combinedLength start1 start2 l1 l2) (f1 ∧ f2) (fun m => (p1 (projVars (start1 - combinedStart start1 start2) l1 m) /\ p2 (projVars (start2 - combinedStart start1 start2) l2 m))). 
+  Proof. 
+    intros G1 G2. 
+    intros a. split; intros H. 
+    + apply evalFormula_and_iff in H as (H1 & H2). 
+      rewrite <- projVars_combined1, <- projVars_combined2. 
+      unfold encodesPredicateAt in G1, G2. rewrite <- G1, <- G2. easy. 
+    + rewrite <- projVars_combined1, <- projVars_combined2 in H. 
+      unfold satisfies. apply evalFormula_and_iff. 
+      split; [apply G1, H | apply G2, H]. 
+  Qed. 
+
+  (*...and with ∨*)
+  Lemma encodesPredicate_or start1 start2 l1 l2 f1 f2 p1 p2 : 
+    encodesPredicateAt start1 l1 f1 p1 -> encodesPredicateAt start2 l2 f2 p2 
+    -> encodesPredicateAt (combinedStart start1 start2) (combinedLength start1 start2 l1 l2) (f1 ∨ f2) (fun m => (p1 (projVars (start1 - combinedStart start1 start2) l1 m) \/ p2 (projVars (start2 - combinedStart start1 start2) l2 m))).
+  Proof. 
+    intros G1 G2. 
+    intros a. split; intros H. 
+    + apply evalFormula_or_iff in H as [H | H]; 
+      rewrite <- projVars_combined1, <- projVars_combined2;
+      unfold encodesPredicateAt in G1, G2; rewrite <- G1, <- G2; easy. 
+    + rewrite <- projVars_combined1, <- projVars_combined2 in H. 
+      unfold satisfies. apply evalFormula_or_iff. 
+      destruct H as [H | H]; [left; apply G1, H | right; apply G2, H].
+  Qed. 
+
+  (*encoding of single literals *)
+  Definition encodeLiteral v (sign : bool) : formula := if sign then v else ¬ v. 
+
+  Lemma encodeLiteral_correct v sign : forall a, satisfies a (encodeLiteral v sign) <-> evalVar a v = sign. 
+  Proof. 
+    intros. unfold satisfies, encodeLiteral. destruct sign; cbn; [ tauto |simp_bool; tauto ]. 
+  Qed. 
+
+  Lemma encodeLiteral_encodesPredicate v sign : encodesPredicateAt v 1 (encodeLiteral v sign) (fun l => l = [sign]). 
+  Proof. 
+    intros. split; intros. 
+    + apply encodeLiteral_correct in H. specialize (explicitAssignment_length a v 1) as H1. 
+      assert (0 < 1) as H2 by lia. 
+      specialize (@explicitAssignment_nth a v 1 0 H2) as H3. 
+      destruct explicitAssignment as [ | s l]; cbn in H1; [ congruence | destruct l; [ | cbn in H1; congruence]]. 
+      cbn in H3. now inv H3. 
+    + apply encodeLiteral_correct. assert (0 < 1) as H2 by lia.
+      specialize (@explicitAssignment_nth a v 1 0 H2) as H1. 
+      rewrite H in H1; cbn in H1. now inv H1. 
+  Qed. 
+
+  (*for predicates which are equivalent, encoding is equivalent *)
+  Lemma encodesPredicateAt_extensional s l f p1 p2 : (forall m, |m| = l -> p1 m <-> p2 m) -> encodesPredicateAt s l f p1 <-> encodesPredicateAt s l f p2. 
+  Proof. 
+    intros. unfold encodesPredicateAt. split; intros; specialize (H (explicitAssignment a s l) (explicitAssignment_length _ _ _)); [now rewrite <- H | now rewrite H]. 
+  Qed. 
+
+  (*a procedure that tries to simplify parts of the terms introduced by the combination lemmas for ∧ and ∨ *)
+  Ltac encodesPredicateAt_comp_simp H := 
+    unfold combinedStart, combinedLength in H;
+    try (rewrite Nat.min_l in H by nia); try (rewrite Nat.min_r in H by nia);
+    try (rewrite Nat.max_l in H by nia); try (rewrite Nat.max_r in H by nia);
+    try rewrite !Nat.sub_diag in H.
+  
+  (*encoding of lists *)
+  Fixpoint encodeListAt (startA : nat) (l : list bool) :=
+    match l with 
+    | [] => Ftrue
+    | x :: l => (encodeLiteral startA x) ∧ (encodeListAt (1 + startA) l)
+    end. 
+
+  Lemma encodeListAt_encodesPredicate start l : encodesPredicateAt start (|l|) (encodeListAt start l) (fun m => m = l).
+  Proof. 
+    revert start. induction l; intros. 
+    - cbn. split; [eauto | ]. unfold satisfies. intros; easy. 
+    - cbn. specialize (@encodesPredicate_and start (S start) 1 (|l|) (encodeLiteral start a) (encodeListAt (S start) l) _ _ (encodeLiteral_encodesPredicate start a) (IHl (S start))) as H1.
+      encodesPredicateAt_comp_simp H1. 
+      replace (S start - start) with 1 in H1 by lia. 
+      replace (S start + (|l|) - start) with (S (|l|)) in H1 by lia.
+      eapply encodesPredicateAt_extensional; [ | apply H1]. 
+      intros m H0. unfold projVars. 
+      destruct m; cbn; [split; intros; easy | ]. 
+      split. 
+      + intros H. inv H. now rewrite firstn_all.
+      + intros (H2 & H3). inv H2. f_equal. apply Nat.succ_inj in H0. now apply firstn_all_inv. 
+  Qed. 
+
+
+  (*encoding of windows *)
+  (*startA is the position at which the premise is placed, startB the position at which the conclusion is placed *)
+  Definition encodeWindowAt (startA startB : nat) (win : PRWin bool) := encodeListAt startA (prem win) ∧ encodeListAt startB (conc win). 
+
+  Lemma encodeWindowAt_encodesPredicate start len win : 
+    win el windows -> encodesPredicateAt start (len + width) (encodeWindowAt start (start + len) win) (fun m => projVars 0 width m = prem win /\ projVars len width m = conc win). 
+  Proof. 
+    intros H0. 
+    specialize (encodesPredicate_and (encodeListAt_encodesPredicate start (prem win)) (encodeListAt_encodesPredicate (start + len) (conc win))) as H. 
+    destruct A as (_ & _ & _ & A0 & A1 & _). apply A1 in H0 as (H0 & H0').
+    encodesPredicateAt_comp_simp H. 
+    rewrite !H0 in H. rewrite !H0' in H.
+    replace (start + len + width - start) with (len + width) in H by lia. 
+    replace (start + len - start) with len in H by lia.
+    unfold encodeWindowAt. eapply encodesPredicateAt_extensional; [ | apply H].
+    tauto.
+  Qed.
+
+  (*encoding of the disjunction of all windows of the BinaryPR instance  *)
+  Definition encodeWindowsAt (startA startB : nat) := listOr (map (encodeWindowAt startA startB) windows). 
+
+  Lemma encodeWindowsAt_encodesPredicate len start : len >= width -> encodesPredicateAt start (len + width) (encodeWindowsAt start (start + len)) (fun m => exists win, win el windows /\ projVars 0 width m = prem win /\ projVars len width m = conc win). 
+  Proof. 
+    intros F0.
+    specialize (encodeWindowAt_encodesPredicate) as H1. 
+    unfold encodeWindowsAt. 
+    induction windows. 
+    - cbn. split. 
+      + unfold satisfies. cbn. congruence. 
+      + intros (win & [] & _). 
+    - cbn. match type of IHl with ?a -> _ => assert a as H by (intros; apply H1; eauto); apply IHl in H; clear IHl end. 
+      specialize (H1 start len a (or_introl eq_refl)). 
+      specialize (encodesPredicate_or H1 H) as H2. clear H1 H. 
+      cbn in H2. 
+      destruct A as (_ & _ & (k & A1 & A2) & _).
+      encodesPredicateAt_comp_simp H2. 
+      replace (start + (len + width) - start) with (len + width) in H2 by lia.
+      eapply encodesPredicateAt_extensional; [ | apply H2]. 
+      intros; cbn. 
+      rewrite !projVars_comp. cbn. rewrite !Nat.min_l by lia. rewrite Nat.add_0_r. 
+      split; intros. 
+      + destruct H0 as (win & [<- | H0] & F1 & F2); [now left | right; eauto].
+      + destruct H0 as [(F1 & F2) | (win & H0 & F1 & F2)]; eauto 7. 
+  Qed. 
+
+  (*encoding of all windows of one line of the tableau *)
+  (*we only need to place a window every offset fields, but subtracting offset isn't structurally recursive *)
+  (*therefore we use a stepindex (initalise to the same value as l) *)
+  Fixpoint encodeWindowsInLine' (stepindex l : nat) (startA startB : nat) := 
+    if l <? width then Ftrue 
+                  else match stepindex with 
+                    | 0 => Ftrue
+                    | S stepindex => encodeWindowsAt startA startB ∧ encodeWindowsInLine' stepindex (l - offset) (startA + offset) (startB + offset)
+                    end.
+
+  Lemma encodeWindowsInLine'_stepindex_monotone' index startA startB : forall n, n <= index -> encodeWindowsInLine' index n startA startB = encodeWindowsInLine' (S index) n startA startB. 
+  Proof. 
+    destruct A as (A1 & A2 & _).
+    revert startA startB.
+    induction index; intros. 
+    - unfold encodeWindowsInLine'. assert (n = 0) as -> by lia. cbn; destruct width; [ lia | easy ].
+    - unfold encodeWindowsInLine'. destruct (Nat.ltb n width); [ easy | ]. fold encodeWindowsInLine'. 
+      erewrite IHindex by lia. easy. 
+  Qed. 
+
+  Lemma encodeWindowsInLine'_stepindex_monotone index index' startA startB : index' >= index -> encodeWindowsInLine' index index startA startB = encodeWindowsInLine' index' index startA startB. 
+  Proof. 
+    intros. revert index H.
+    induction index'; intros. 
+    - assert (index = 0) as -> by lia. easy.
+    - destruct (nat_eq_dec (S index') index). 
+      + now rewrite e.
+      + assert (index' >= index) as H1 by lia. rewrite <- encodeWindowsInLine'_stepindex_monotone' by lia. now apply IHindex'.
+  Qed.
+
+  Lemma encodeWindowsInLine'_encodesPredicate start l : l <= llength -> (exists k, l = k * offset) -> encodesPredicateAt start (l + llength) (encodeWindowsInLine' l l start (start + llength)) (fun m => valid offset width windows (projVars 0 l m) (projVars llength l m)). 
+  Proof. 
+    intros A0.
+    (*need strong induction *)
+    destruct A as (A1 & A4 & A2 & A5 & A7 & A3). 
+    revert start A0.  
+    apply complete_induction with (x := l). clear l. intros l IH. intros. 
+
+    (*case analysis on the stepindex *)
+    destruct l.
+    - (*we use that width > 0 *)
+      unfold encodeWindowsInLine'. rewrite (proj2 (Nat.ltb_lt _ _) A1). 
+      intros a. split; [ intros; constructor | intros _; unfold satisfies; eauto].  
+    - destruct (le_lt_dec width (S l)). 
+      + assert (~ (S l) < width) as H3%Nat.ltb_nlt by lia. cbn -[projVars]; setoid_rewrite H3. 
+        destruct offset as [ | offset]; [ lia | ].
+        (* we use the IH for l - offset *)
+ 
+        assert (S l - S offset < S l) as H1 by lia. apply IH with (start := start + S offset) in H1. 2: nia. 
+        2: { destruct H as (k & H). destruct k; [ lia | ]. exists k. lia. }
+        clear H IH. 
+        assert (llength >= width) as H0 by lia.
+        apply (encodeWindowsAt_encodesPredicate start) in H0. 
+
+        specialize (encodesPredicate_and H0 H1) as H2. clear H1 H0.
+        encodesPredicateAt_comp_simp H2. 
+
+        replace (start + S offset + llength) with (start + llength + S offset) in H2 by lia. 
+        replace (start + S offset + (l - offset + llength) - start) with (S (l + llength)) in H2. 
+        2: { destruct A2 as (? & A2 & A6). nia. }
+        
+        rewrite encodeWindowsInLine'_stepindex_monotone with (index' := l) in H2; [ | lia].
+        eapply encodesPredicateAt_extensional; [ | apply H2].
+
+        clear H2 H3. 
+        intros. 
+        destruct A2 as (k & A2 & A2').
+        assert (S l = S offset + (S l - S offset)) as H0 by nia.  
+        (*we now show the two directions of the equivalence, which is a bit technical*)
+        split; intros. 
+        * rewrite H0 in H1. clear H0. 
+          rewrite !projVars_add in H1. inv H1.
+          (*the first two cases are contradictory *)
+          2 : { exfalso. apply list_eq_length in H0. rewrite !app_length in H0. rewrite !projVars_length in H0; [ | easy | easy]. nia. }
+          1: { exfalso. apply list_eq_length in H3. rewrite !app_length in H3. rewrite projVars_length in H3; [ | cbn; nia]. cbn in H3. lia. } 
+
+          apply app_eq_length in H2 as (-> & ->); [ | rewrite projVars_length; [easy | nia] ].
+          apply app_eq_length in H0 as (-> & ->); [ | rewrite projVars_length; [easy | nia]]. 
+          split.
+          -- exists win. rewrite !projVars_comp; cbn. rewrite !Nat.min_l by lia. 
+             rewrite !Nat.add_0_r.
+             clear H3 H4 H5. rewrite <- !projVars_add in H7. 
+             replace (S offset + (l - offset)) with (width + (S l - width)) in H7 by nia. 
+             rewrite !projVars_add in H7.
+             split; [ easy | split ]; apply A7 in H6 as (H6 & H6'). 
+             ++ destruct H7 as ((b & H7) & _). eapply app_eq_length in H7; [ easy| rewrite projVars_length; easy ]. 
+             ++ destruct H7 as (_ & (b & H7)). eapply app_eq_length in H7; [ easy | rewrite projVars_length; easy].
+          -- clear H7 H6. 
+             rewrite !projVars_comp. replace (start + S offset - start) with (S offset) by lia. rewrite !Nat.min_l by lia. 
+             apply H3. 
+        * (*other direction of the equivalence *)
+          destruct H1 as (H1 & H2).  
+          rewrite H0, !projVars_add. 
+          destruct H1 as (win & H1 & F1 & F2). 
+          econstructor 3. 
+          -- rewrite !projVars_comp in H2. rewrite !Nat.min_l in H2 by lia.
+             replace (start + S offset - start) with (S offset) in H2 by lia. 
+             apply H2. 
+          -- rewrite projVars_length; lia. 
+          -- rewrite projVars_length; lia. 
+          -- clear H2. apply H1. 
+          -- clear H2. rewrite <- !projVars_add. 
+             replace (S offset + (S l - S offset)) with (width + (S l - width)) by lia. 
+             rewrite !projVars_add. 
+             rewrite projVars_comp in F1, F2. rewrite !Nat.min_l in F1, F2 by lia. 
+             rewrite Nat.add_0_r in F2; cbn in F1, F2.
+             rewrite F1, F2. split; unfold prefix; eauto. 
+    + (*the case where the remaining string is too short for a rewrite window to hold - validity holds vacuously *)
+      clear IH. assert ( (S l) < width) as H3%Nat.ltb_lt by lia. cbn -[projVars]; setoid_rewrite H3.
+      intros a; split; [intros _ | ]. 
+      * destruct H as (k & H). eapply valid_vacuous. 
+        -- rewrite !projVars_length; [easy | rewrite explicitAssignment_length; lia | rewrite explicitAssignment_length; lia]. 
+        -- rewrite projVars_length; [ easy | rewrite explicitAssignment_length; lia]. 
+        -- rewrite projVars_length; [ | rewrite explicitAssignment_length; lia]. 
+           (*here we need the assumption that l is a multiple of offset *)
+           apply H. 
+      * intros _; easy. 
+  Qed.
+
+  (*the above construction specialized to the setting we need: the conclusion starts exactly one line after the premise *)
+  Definition encodeWindowsInLine start := encodeWindowsInLine' llength llength start (start + llength). 
+  Lemma encodeWindowsInLine_encodesPredicate start : encodesPredicateAt start (llength + llength) (encodeWindowsInLine start) (fun m => valid offset width windows (projVars 0 llength m) (projVars llength llength m)). 
+  Proof. 
+    unfold encodeWindowsInLine.
+    apply (@encodeWindowsInLine'_encodesPredicate start llength); [easy | apply A].
+  Qed. 
+
+  (*encoding of windows in all lines of the tableua *)
+  Fixpoint encodeWindowsInAllLines' (start : nat) (t : nat)  := 
+    match t with 
+    | 0 => Ftrue
+    | S t => encodeWindowsInLine start ∧ encodeWindowsInAllLines' (start + llength) t
+    end. 
+
+  Definition encodeWindowsInAllLines := encodeWindowsInAllLines' 0 steps. 
+
+  Lemma encodeWindowsInAllLines'_encodesPredicate start : encodesPredicateAt start ((S steps) * llength) (encodeWindowsInAllLines' start steps) 
+    (fun m => (forall i, 0 <= i < steps -> valid offset width windows (projVars (i * llength) llength m) (projVars (S i * llength) llength m))). 
+  Proof. 
+    revert start. induction steps; cbn; intros. 
+    - rewrite !Nat.add_0_r. 
+      intros a; unfold satisfies; cbn; split; [ intros _; intros; lia | easy]. 
+    - specialize (encodeWindowsInLine_encodesPredicate start) as H1. 
+      specialize (IHn (start + llength)). 
+      specialize (encodesPredicate_and H1 IHn) as H. clear IHn H1. 
+
+      encodesPredicateAt_comp_simp H. 
+      replace (start + llength + S n * llength - start) with (llength + (llength + n * llength)) in H by lia. 
+      replace (start + llength - start) with llength in H by lia. 
+
+      eapply encodesPredicateAt_extensional; [ | apply H].
+      clear H. intros m. cbn -[projVars]. 
+      rewrite !projVars_comp. setoid_rewrite projVars_comp. cbn. rewrite !Nat.min_l by lia. 
+      rewrite Nat.add_0_r. split. 
+      + intros H1. split.
+        * specialize (H1 0). cbn in H1. rewrite Nat.add_0_r in H1. apply H1; lia.
+        * intros i H2. 
+          specialize (H1 (S i)). cbn in H1. rewrite Nat.add_comm. rewrite <- Nat.add_assoc. 
+          rewrite !Nat.min_l by nia.  setoid_rewrite Nat.add_comm at 3.
+          apply H1. lia.
+      + intros (H1 & H2). intros i H3. destruct i. 
+        * cbn. rewrite Nat.add_0_r. apply H1.
+        * specialize (H2 i). 
+          rewrite !Nat.min_l in H2 by nia.
+          cbn. rewrite Nat.add_comm. rewrite Nat.add_assoc. now apply H2. 
+  Qed.
+
+  (*again a version specialised to our needs *)
+  Corollary encodeWindowsInAllLines_encodesPredicate : encodesPredicateAt 0 ((S steps) * llength) encodeWindowsInAllLines 
+    (fun m => (forall i, 0 <= i < steps -> valid offset width windows (projVars (i * llength) llength m) (projVars (S i * llength) llength m))). 
+  Proof. 
+    unfold encodeWindowsInAllLines. apply encodeWindowsInAllLines'_encodesPredicate. 
+  Qed. 
+
+  (*encode the substring constraint for a single string s *)
+  (*should only be called for s satisfying |s| > 0; for s = nil, the breaking condition does not work as intended*)
+  (*in principle, this is not a problem as the resulting formula is still equivalent to the desired formula, but this breaks monotonicity*)
+  Fixpoint encodeSubstringInLine' (s : list bool) (stepindex l : nat) (start : nat) := 
+    if l <? |s| then Ffalse
+                  else match stepindex with 
+                    | 0 => (match s with [] => Ftrue | _ => Ffalse end)
+                    | S stepindex => encodeListAt start s ∨ encodeSubstringInLine' s stepindex (l - offset) (start + offset) 
+                    end.
+
+  (*the requirement |s| > 0 is needed for monotonicity *)
+  Lemma encodeSubstringInLine'_stepindex_monotone' s index start : forall n, |s| > 0 -> n <= index -> encodeSubstringInLine' s index n start = encodeSubstringInLine' s (S index) n start. 
+  Proof. 
+    destruct A as (A1 & A2 & _).
+    revert start.
+    induction index; intros. 
+    - unfold encodeSubstringInLine'. assert (n = 0) as -> by lia. cbn; destruct s; [ cbn in *; lia | easy ]. 
+    - unfold encodeSubstringInLine'. destruct (Nat.ltb n (|s|)); [ easy | ]. fold encodeSubstringInLine'. 
+      erewrite IHindex by lia. easy. 
+  Qed. 
+
+  Lemma encodeSubstringInLine'_stepindex_monotone s index1 index2 start : 
+    |s| > 0 -> index2 >= index1 -> encodeSubstringInLine' s index1 index1 start = encodeSubstringInLine' s index2 index1 start.
+  Proof. 
+    intros. revert index1 H0. 
+    induction index2; intros.
+    - assert (index1 = 0) as -> by lia. easy.
+    - destruct (nat_eq_dec (S index2) index1). 
+      + now rewrite e.
+      + assert (index2 >= index1) as H1 by lia. rewrite <- encodeSubstringInLine'_stepindex_monotone' by lia. now apply IHindex2.
+  Qed. 
+
+  Lemma encodeSubstringInLine'_encodesPredicate s start l : |s| > 0 -> l <= llength 
+    -> (exists k, l = k * offset) -> encodesPredicateAt start l (encodeSubstringInLine' s l l start) (fun m => (exists k, k * offset <= l /\ projVars (k * offset) (|s|) m = s)). 
+  Proof. 
+    intros F.
+    (*need strong induction *)
+    destruct A as (A1 & A4 & A2 & A5 & A7 & A3). 
+    revert start.  
+    apply complete_induction with (x := l). clear l. intros l IH. intros. 
+
+    destruct l.
+    - cbn -[projVars]. destruct s; cbn -[projVars]. 
+      + (*trivially true because of our requirement that |s| > 0*) cbn in F; easy. 
+      + (*trivially false *)
+        intros a; split.
+        * unfold satisfies; cbn; congruence. 
+        * intros (k & H1 & H2). destruct k; [clear H1 | nia]. cbn in H2. congruence. 
+    - destruct (le_lt_dec (|s|) (S l)). 
+      + (*in this case, we can apply the IH*)
+        assert (~ (S l) < (|s|)) as H3%Nat.ltb_nlt by lia. cbn -[projVars]; setoid_rewrite H3. 
+        destruct offset as [ | offset]; [ lia | ].
+        (* we use the IH for l - offset *)
+ 
+        assert (S l - S offset < S l) as H1 by lia. apply IH with (start := start + S offset) in H1; [ | nia | ]. 
+        2: { destruct H0 as (k & H0). destruct k; [ lia | ]. exists k. lia. }
+        clear H IH. 
+        specialize (encodeListAt_encodesPredicate start s) as H2.
+        specialize (encodesPredicate_or H2 H1) as H. clear H1 H2 H3.
+
+        encodesPredicateAt_comp_simp H.
+        destruct H0 as (k & H0).
+        assert (k > 0) by nia. (*a hint for nia - without it, the following replace will not work *)
+        replace (start + S offset + (S l - S offset) - start) with (S l) in H by nia.
+        replace (start + S offset - start) with (S offset) in H by lia.
+
+        rewrite encodeSubstringInLine'_stepindex_monotone with (index2 := l) in H; [ | apply F| lia].
+        eapply encodesPredicateAt_extensional; [ | apply H]. clear H.
+        intros. cbn. split.
+        * intros (k0 & H2 & H3). 
+          destruct k0; [ now left | right]. 
+          exists k0. split; [ easy | ]. 
+          rewrite projVars_comp. 
+          cbn [Nat.mul] in H3.  
+          enough (|s| <= l - offset - k0 * S offset).
+          { rewrite Nat.min_l by lia. rewrite Nat.add_comm. apply H3. }
+          apply projVars_in_ge in H3; nia.
+        * intros H3. 
+          destruct H3 as [H3 | (k0 & H3 & H4)]; [ exists 0; cbn; easy | ]. 
+          exists (S k0). split; [ nia | ].
+          rewrite projVars_comp in H4. 
+
+          enough (|s| <= l - offset - k0 * S offset).
+          { rewrite Nat.min_l in H4 by lia. cbn [Nat.mul]. rewrite <- Nat.add_comm. apply H4. }
+          apply list_eq_length in H4. 
+          match type of H4 with (|projVars ?a ?b ?c| = _) => specialize (projVars_length_le2 a b c) as H2 end.
+          lia. 
+    + (*the case where the remaining string is too short in order to place the substring constraint *)
+      clear IH. assert ( (S l) < (|s|)) as H3%Nat.ltb_lt by lia. cbn -[projVars]; setoid_rewrite H3.
+      intros a. unfold satisfies; cbn [negb evalFormula].
+      split; [congruence | ]. 
+      intros (k & H1 & H2). apply list_eq_length in H2. specialize (projVars_length_le (k * offset) (|s|) (explicitAssignment a start (S l))) as H4.
+      rewrite explicitAssignment_length in H4. lia. 
+  Qed.
+
+  (*TODO: consistent argument order over all functions *)
+
+  (*we now have to do a case analysis: if the substring which has to be checked is non-empty, we use the function defined above *)
+  (*otherwise, the empty string is trivially a substring *)
+  Definition encodeSubstringInLine s start l := match s with [] => Ftrue | _ => encodeSubstringInLine' s l l start end.
+
+  Lemma encodeSubstringInLine_encodesPredicate s start l : l <= llength -> (exists k, l = k * offset) -> encodesPredicateAt start l (encodeSubstringInLine s start l) (fun m => (exists k, k * offset <= l /\ projVars (k * offset) (|s|) m = s)). 
+  Proof. 
+    intros. unfold encodeSubstringInLine. destruct s eqn:H1. 
+    - unfold satisfies. cbn. intros; split.
+      + intros _. exists 0; cbn; firstorder.
+      + intros _. reflexivity. 
+    - apply encodeSubstringInLine'_encodesPredicate; cbn; easy.
+  Qed. 
+
+  (*the final constraint now is a disjunction over all given substrings *)
+  Definition encodeFinalConstraint (start : nat) := listOr (map (fun s => encodeSubstringInLine s start llength) final). 
+
+  Lemma encodesPredicate_listOr (X : Type) (l : list X) (encode : X -> nat -> nat -> formula) (p : X -> list bool -> Prop) start len : 
+    (forall x, x el l -> encodesPredicateAt start len (encode x start len) (p x)) 
+   -> encodesPredicateAt start len (listOr (map (fun x => encode x start len) l)) (fun m => (exists x, x el l /\ p x m)). 
+  Proof. 
+    intros H. induction l. 
+    - cbn. intros a. unfold satisfies; cbn. split; [ congruence | intros (_ & [] & _)].
+    - specialize (IHl (fun x Hel => H x (or_intror Hel))). cbn. 
+      specialize (H a (or_introl eq_refl)). 
+      specialize (encodesPredicate_or H IHl) as H1. clear IHl H. 
+      encodesPredicateAt_comp_simp H1. 
+      replace (start + len - start) with len in H1 by lia. 
+
+      eapply encodesPredicateAt_extensional; [ clear H1| apply H1].
+      intros m H2; split.
+      + intros (x & [-> | H] & H1). 
+        * left; now rewrite projVars_all.
+        * right. rewrite projVars_all; easy. 
+      + intros [H | (x & H & H')].
+        * exists a. now rewrite projVars_all in H.
+        * exists x. rewrite projVars_all in H'; easy.
+  Qed. 
+
+  Lemma encodeFinalConstraint_encodesPredicate start : encodesPredicateAt start llength (encodeFinalConstraint start) (fun m => satFinal offset llength final m).
+  Proof. 
+    unfold encodeFinalConstraint. 
+    eapply encodesPredicateAt_extensional; [ | apply encodesPredicate_listOr]. 
+    2: { intros. apply encodeSubstringInLine_encodesPredicate; [easy | apply A]. }
+    intros m H4. split. 
+    - intros (subs & k & H1 & H2 & H3).
+      exists subs. split; [ apply H1 | ]. 
+      exists k. split; [ easy | ]. 
+      destruct H3 as (b & H3). unfold projVars. rewrite H3. 
+      rewrite firstn_app, firstn_all, Nat.sub_diag; cbn. now rewrite app_nil_r. 
+    - intros (subs & H1 & (k & H2 & H3)).
+      exists subs, k. split; [apply H1 | split; [ apply H2 | ]].
+      unfold prefix. unfold projVars in H3. 
+      setoid_rewrite <- firstn_skipn with (l := skipn (k * offset) m) (n:= |subs|).
+      setoid_rewrite H3. eauto.
+  Qed. 
+
+  (*encoding of the whole tableau: the initial constraint, window constraints and the final constraint are combined conjunctively *)
+  Definition encodeTableau := encodeListAt 0 init ∧ encodeWindowsInAllLines ∧ encodeFinalConstraint (steps * llength).
+  Lemma encodeTableau_encodesPredicate : 
+    encodesPredicateAt 0 (S steps * llength) encodeTableau 
+    (fun m => projVars 0 llength m = init 
+      /\ (forall i, 0 <= i < steps -> valid offset width windows (projVars (i * llength) llength m) (projVars (S i * llength) llength m)) 
+      /\ satFinal offset llength final (projVars (steps * llength) llength m)). 
+  Proof. 
+    specialize (encodesPredicate_and (encodeListAt_encodesPredicate 0 init) encodeWindowsInAllLines_encodesPredicate) as H. 
+    encodesPredicateAt_comp_simp H.  
+    specialize (encodesPredicate_and H (encodeFinalConstraint_encodesPredicate (steps * llength))) as H1.
+    clear H. 
+    encodesPredicateAt_comp_simp H1. 
+    unfold encodeTableau. 
+    replace (llength + steps * llength - 0 - 0) with (S steps * llength) in H1 by lia.
+
+    eapply encodesPredicateAt_extensional; [ clear H1| apply H1].
+    intros m H4. 
+    setoid_rewrite projVars_comp. rewrite !Nat.min_l by nia. 
+    setoid_rewrite Nat.add_0_r. setoid_rewrite Nat.sub_0_r. 
+    split. 
+    - intros (H1 & H2 & H3). 
+      repeat split; [easy | | easy].
+      intros. rewrite !Nat.min_l by nia. rewrite !projVars_comp. rewrite !Nat.min_l by nia. 
+      rewrite !Nat.add_0_r. now apply H2.
+    - rewrite !and_assoc. intros (H1 & H2 & H3). split; [easy |split;[ | easy]]. 
+      intros. specialize (H2 i H). rewrite !Nat.min_l in H2 by nia. 
+      rewrite !projVars_comp in H2. rewrite !Nat.min_l in H2 by nia.
+      rewrite !Nat.add_0_r in H2. apply H2.
+  Qed. 
+ 
+  (*from a proof that a sequence of rewrites is valid, we can restore a satisfying assignment for the encoded windows of the tableau (by concatenating the strings encountered during the sequence of rewrites)*)
   Lemma relpower_valid_to_assignment n x y: 
     relpower (valid offset width windows) n x y -> |x| = llength 
     -> exists m, |m| = (S n * llength) /\ projVars 0 llength m = x /\ projVars (n * llength) llength m = y 
@@ -788,16 +700,18 @@ Section fixInstance.
           cbn. rewrite !projVars_app3; [ | easy | easy].  apply H7.
   Qed. 
   
+  (*the reduction equivalence for the wellformed BinaryPR instance *)
   Lemma reduction_wf : FSAT encodeTableau <-> exists sf, relpower (valid offset width windows) steps init sf /\ satFinal offset llength final sf. 
   Proof with (try (solve [rewrite explicitAssignment_length; cbn; nia | cbn; lia])). 
-    specialize (encodeTableau_encodesPredicate) as (H1 & H2). split; intros. 
-    - destruct H as (a & H). apply H2 in H as (H3 & H4 & H5). clear H2. rewrite Nat.add_0_r in *. 
+    specialize (encodeTableau_encodesPredicate) as H1. split; intros. 
+    - destruct H as (a & H). apply H1 in H as (H3 & H4 & H5). 
       exists (projVars (steps * llength) llength (explicitAssignment a 0 (S steps * llength))). 
       split; [ | apply H5]. rewrite <- H3. clear H1 H3 H5. 
 
       cbn. rewrite projVars_length... rewrite explicitAssignment_app at 1... rewrite projVars_app1...
       rewrite Nat.add_comm. rewrite explicitAssignment_app, projVars_app2, projVars_all... 
 
+      (*as the assignment is constructed by appending new lines, we use the reversed version of relpower *)
       apply relpower_relpowerRev. induction steps. 
       + cbn. constructor. 
       + econstructor. 
@@ -824,7 +738,7 @@ Section fixInstance.
     - destruct H as (sf & H3 & H4). unfold encodeTableau in *. 
       specialize (relpower_valid_to_assignment H3 eq_refl) as (expAssgn & H5 & H6 & H7 & H8). 
       destruct (expAssgn_to_assgn 0 expAssgn) as (a & H9).
-      exists a. apply H2. clear H2. 
+      exists a. apply H1. clear H1. 
       apply expAssgn_to_assgn_inv in H9. rewrite H5 in H9. rewrite H9. easy.
   Qed. 
 End fixInstance.
@@ -853,6 +767,7 @@ Proof.
   - apply Nat.mod_divide; [ lia | ]. apply H4. 
 Qed. 
 
+(*non-wellformed instances are mapped to a trivial no-instance *)
 Definition trivialNoInstance := 0 ∧ ¬0. 
 Lemma trivialNoInstance_isNoInstance : not (FSAT trivialNoInstance). 
 Proof. 
